shift-reset/interpreter/imonad.v
@@ -33,6 +33,14 @@ Definition imonad_map {A B} (f : A -> B) (m : imonad A) :=
             | inr x => (inr (f x), h)
             end).
 
+Definition imonad_replace {A B} (x : A) (m : imonad B) : imonad A :=
+  IMonad (fun env h =>
+            let (r, h) := imonad_run m env h in
+            match r with
+            | inl e => (inl e, h)
+            | inr _ => (inr x, h)
+            end).
+
 Definition imonad_pure {A} (x : A) : imonad A :=
   IMonad (fun _ h => (inr x, h)).
 
@@ -41,12 +49,11 @@ Definition imonad_lift2 {A B C} (f : A -> B -> C) (m1 : imonad A) (m2 : imonad B
             let (r, h) := imonad_run m1 env h in
             match r with
             | inl e => (inl e, h)
-            | inr x =>
-                let (r, h) := imonad_run m2 env h in
-                match r with
-                | inl e => (inl e, h)
-                | inr y => (inr (f x y), h)
-                end
+            | inr x => let (r, h) := imonad_run m2 env h in
+                       match r with
+                       | inl e => (inl e, h)
+                       | inr y => (inr (f x y), h)
+                       end
             end).
 
 Definition imonad_bind {A B} (m : imonad A) (f : A -> imonad B) : imonad B :=
@@ -70,3 +77,19 @@ Definition imonad_eval {A} (m : imonad A) (env : env) (h : iheap) : ierror + A :
 
 Definition imonad_exec {A} (m : imonad A) (env : env) (h : iheap) : iheap :=
   snd (imonad_run m env h).
+
+Definition imonad_kleisli_compose {A B C} (f1 : A -> imonad B) (f2 : B -> imonad C) (x : A) : imonad C :=
+  imonad_bind (f1 x) f2.
+
+Declare Scope imonad_scope.
+Delimit Scope imonad_scope with imonad.
+Bind Scope imonad_scope with imonad.
+
+Notation "f <$> m" := (imonad_map f m) (at level 65, left associativity) : imonad_scope.
+Notation "x <$ m" := (imonad_replace x m) (at level 65, left associativity) : imonad_scope.
+Notation "m >>= f" := (imonad_bind m f) (at level 60, right associativity) : imonad_scope.
+Notation "m1 >> m2" := (imonad_then m1 m2) (at level 60, right associativity) : imonad_scope.
+Notation "f1 >=> f2" := (imonad_kleisli_compose f1 f2) (at level 60, right associativity) : imonad_scope.
+
+Notation "x <- m1 ; m2" := (imonad_bind m1 (fun x => m2)) (at level 100, right associativity) : imonad_scope.
+Notation "m1 ;; m2" := (imonad_then m1 m2) (at level 100, right associativity) : imonad_scope.
